tests/lean/tacUnsolvedGoalsErrors.lean
@@ -1,0 +1,34 @@
+theorem ex1 (p q r : Prop) (h1 : p ∨ q) (h2 : p → q) : q :=
+  have q by -- Error here
+    skip
+  by skip -- Error here
+     skip
+
+theorem ex2 (p q r : Prop) (h1 : p ∨ q) (h2 : p → q) : q :=
+  have q by {
+    skip
+  } -- Error here
+  by skip -- Error here
+     skip
+
+theorem ex3 (p q r : Prop) (h1 : p ∨ q) (h2 : p → q) : q := by
+  cases h1
+  { skip
+    skip } -- Error here
+  { skip
+    skip } -- Error here
+
+theorem ex4 (p q r : Prop) (h1 : p ∨ q) (h2 : p → q) : q := by
+  first | done | apply ex3 p q r h1 h2
+
+syntax "." tacticSeq : tactic
+
+macro_rules
+  | `(tactic| .%$dot $ts:tacticSeq) => `(tactic| { ($ts:tacticSeq) }%$dot)
+
+theorem ex5 (p q r : Prop) (h1 : p ∨ q) (h2 : p → q) : q := by
+  cases h1
+  . skip  -- Error here
+    skip
+  . skip  -- Error here
+    skip
